\documentclass[12pt,a4paper,twocolumn]{article}
% The following LaTeX packages must be installed on your machine: amsmath, authblk, bm, booktabs, caption, dcolumn, fancyhdr, geometry, graphicx, hyperref, latexsym, natbib
\input{151.dat}
\usepackage{gensymb}
\usepackage{amsthm}
\usepackage{float}
\usepackage{siunitx}
\usepackage{amssymb}
\usepackage{float}
\usepackage{enumerate}
\usepackage{listings}
\usepackage{mathtools}
\PassOptionsToPackage{hyphens}{url}\usepackage{hyperref}
\usepackage[none]{hyphenat}
\usepackage{physics}
%\renewcommand{\familydefault}{\sfdefault}


\begin{document}

\setcounter{page}{1}

\section*{PS 43: Problem 4.21}
\bigskip

Given the following:

\begin{align}
	\frac{1}{T} &= -k\frac{1}{2\mu B}\ln\qty(\frac{N-n}{n}) \label{eq:given-t} \\
	E &= -(2n - N)\mu B \label{eq:given-e}
\end{align}

Solving for $n/N$ in \eqref{eq:given-t}:

\begin{align}
	-\frac{2\mu B}{kT} &= \ln\qty(\frac{N - n}{n}) \\
	e^{-2\mu B/kT} &= \frac{N-n}{n} \\
	e^{-2\mu B/kT} &= \frac{N}{n} - 1 \\
	1 + e^{-2\mu B/kT} &= \frac{N}{n} \\
	\Aboxed{
		\frac{n}{N} &= \frac{1}{1 + e^{-2\mu B/kT}}
	} \label{eq:answer-1}
\end{align}

Let $\beta \equiv 1/kT$. With some further manipulation:

\begin{align}
	\frac{n}{N} &= \frac{1}{1 + e^{-2\beta\mu B}} \cdot \frac{e^{\beta\mu B}}{e^{\beta\mu B}} \\
	\Aboxed{
	\frac{n}{N} &= \frac{e^{\beta\mu B}}{e^{\beta\mu B} + e^{-\beta\mu B}}
	} \label{eq:answer-2}
\end{align}

which is the same form obtained in GT (4.74b). Solving for $n/N$ in \eqref{eq:given-e}:

\begin{align}
	E &= -(2n - N)\mu B \cdot \frac{N}{N} \\
	&= -\frac{2n - N}{N}N\mu B \\
	&= -\qty(\frac{2n}{N} - 1)N\mu B
\end{align}

Substitute \eqref{eq:answer-1} into this:

\begin{align}
	E &= -\qty(2\frac{e^{\beta\mu B}}{e^{\beta\mu B} + e^{-\beta\mu B}} - 1)N\mu B \\
	&= -\qty(\frac{2e^{\beta\mu B} - e^{\beta\mu B} - e^{-\beta\mu B} }{e^{\beta\mu B} + e^{-\beta\mu B}})N\mu B \\
	&= -\qty(\frac{e^{\beta\mu B} - e^{-\beta\mu B} }{e^{\beta\mu B} + e^{-\beta\mu B}})N\mu B
\end{align}

which can be simplified using the relation $\tanh(x) \equiv \frac{e^{x} - e^{-x} }{e^{x} + e^{-x}}$:

\begin{align}
	E &= -\tanh(\beta\mu B)N\mu B \\
	\Aboxed{
		E &= -N\mu B\tanh(\frac{\mu B}{kT})
	} \label{eq:answer-3}
\end{align}

which is the same form as that in GT (4.73).

\end{document}